lib/everparse/3d/EverParse3d.Actions.Base.fst
@@ -7,6 +7,7 @@ open EverParse3d.Prelude
 open Pulse.Lib.Pervasives
 module I = EverParse3d.InputStream.Base
 module CP = EverParse3d.CopyBuffer
+module R = Pulse.Lib.Reference
 
 module PA = EverParse3d.ProbeActions
 module AppCtxt = EverParse3d.AppCtxt
@@ -2941,32 +2942,33 @@ fn probe_then_validate
     let b = PA.run_probe_m error_handler_macro m typename fieldname "probe" ctxt error_handler_fn src64 prep_dest_sz dest;
     with cd vd . assert (CP.pts_to #_ #base_t #len_t #pos_t dest cd vd);
     if (b <> 0uL) {
-      rewrite (CP.pts_to #_ #base_t #len_t #pos_t dest cd vd)
-        as (I.pts_to
-              (CP.base_of #_ #base_t #len_t #pos_t dest)
-              (CP.len_of #_ #base_t #len_t #pos_t dest)
-              (CP.pos_of #_ #base_t #len_t #pos_t dest)
-              cd vd);
       (* Validate the probed bytes from the beginning of the copy buffer, as
          the Low* interpreter does by passing the validator the position
          `0uL`. Here the position belongs to the buffer, which is reused
          across probe sites, so it has to be rewound explicitly. *)
+      unfold (CP.pts_to #_ #base_t #len_t #pos_t dest cd vd);
       CP.reset #_ #base_t #len_t #pos_t dest cd vd;
+      with d . assert (
+        R.pts_to (CP.descr #_ #base_t #len_t #pos_t dest) d **
+        I.pts_to #base_t #len_t #pos_t
+          (CP.base_of #_ #base_t #len_t #pos_t d)
+          (CP.len_of #_ #base_t #len_t #pos_t d)
+          (CP.pos_of #_ #base_t #len_t #pos_t d) cd cd);
+      (* Read the descriptor out of the handle. The probe may have repointed
+         it, so the triple has to come from the reference rather than from a
+         pure projection of `dest`. *)
+      let dv = !(CP.descr #_ #base_t #len_t #pos_t dest);
       let res = v ctxt error_handler_fn
-        (CP.base_of #_ #base_t #len_t #pos_t dest)
-        (CP.len_of #_ #base_t #len_t #pos_t dest)
-        (CP.pos_of #_ #base_t #len_t #pos_t dest)
+        (CP.base_of #_ #base_t #len_t #pos_t dv)
+        (CP.len_of #_ #base_t #len_t #pos_t dv)
+        (CP.pos_of #_ #base_t #len_t #pos_t dv)
         _ cd cd;
-      with vd' . assert (I.pts_to
-              (CP.base_of #_ #base_t #len_t #pos_t dest)
-              (CP.len_of #_ #base_t #len_t #pos_t dest)
-              (CP.pos_of #_ #base_t #len_t #pos_t dest)
-              cd vd');
-      rewrite (I.pts_to
-              (CP.base_of #_ #base_t #len_t #pos_t dest)
-              (CP.len_of #_ #base_t #len_t #pos_t dest)
-              (CP.pos_of #_ #base_t #len_t #pos_t dest)
-              cd vd')
+      with vd' . assert (I.pts_to #base_t #len_t #pos_t
+              (CP.base_of #_ #base_t #len_t #pos_t dv)
+              (CP.len_of #_ #base_t #len_t #pos_t dv)
+              (CP.pos_of #_ #base_t #len_t #pos_t dv) cd vd');
+      fold (CP.pts_to #_ #base_t #len_t #pos_t dest cd vd');
+      rewrite (CP.pts_to #_ #base_t #len_t #pos_t dest cd vd')
         as (copy_buffer_state #_ #base_t #len_t #pos_t dest
               (Ghost.reveal cd, Ghost.reveal vd'));
       forevery_state_dict_singleton_fold dest_name
