lib/everparse/3d/EverParse3d.ProbeActions.fst
@@ -1,6 +1,8 @@
 module EverParse3d.ProbeActions
 #lang-pulse
 
+module R = Pulse.Lib.Reference
+
 let probe_fn_incremental
   (#copy_buffer_t: Type0)
   (#base_t #len_t #pos_t: Type0)
@@ -203,24 +205,24 @@ ensures exists* v_ctxt' .
       pts_to ctxt v_ctxt' **
       CB.pts_to #_ #base_t #len_t #pos_t dest contents_dest v_dest
 {
-  rewrite (CB.pts_to #_ #base_t #len_t #pos_t #inst #cb_inst dest contents_dest v_dest)
-    as (I.pts_to #base_t #len_t #pos_t
-          (CB.base_of #_ #base_t #len_t #pos_t dest)
-          (CB.len_of #_ #base_t #len_t #pos_t dest)
-          (CB.pos_of #_ #base_t #len_t #pos_t dest)
-          contents_dest v_dest);
+  unfold (CB.pts_to #_ #base_t #len_t #pos_t #inst #cb_inst dest contents_dest v_dest);
+  with d . assert (
+    R.pts_to (CB.descr #_ #base_t #len_t #pos_t dest) d **
+    I.pts_to #base_t #len_t #pos_t
+      (CB.base_of #_ #base_t #len_t #pos_t d)
+      (CB.len_of #_ #base_t #len_t #pos_t d)
+      (CB.pos_of #_ #base_t #len_t #pos_t d)
+      contents_dest v_dest);
+  (* The descriptor has to be read out of the handle: a probe may have
+     repointed the copy buffer. *)
+  let dv = !(CB.descr #_ #base_t #len_t #pos_t dest);
   ((if use_error_handler then err else error_handler_macro) <: error_handler #base_t #len_t #pos_t #inst)
     tn fn_ det 0uy ctxt
-      (CB.base_of #_ #base_t #len_t #pos_t dest)
-      (CB.len_of #_ #base_t #len_t #pos_t dest)
-      (CB.pos_of #_ #base_t #len_t #pos_t dest)
+      (CB.base_of #_ #base_t #len_t #pos_t dv)
+      (CB.len_of #_ #base_t #len_t #pos_t dv)
+      (CB.pos_of #_ #base_t #len_t #pos_t dv)
       contents_dest v_dest;
-  rewrite (I.pts_to #base_t #len_t #pos_t
-          (CB.base_of #_ #base_t #len_t #pos_t dest)
-          (CB.len_of #_ #base_t #len_t #pos_t dest)
-          (CB.pos_of #_ #base_t #len_t #pos_t dest)
-          contents_dest v_dest)
-    as (CB.pts_to #_ #base_t #len_t #pos_t #inst #cb_inst dest contents_dest v_dest);
+  fold (CB.pts_to #_ #base_t #len_t #pos_t #inst #cb_inst dest contents_dest v_dest);
 }
 
 inline_for_extraction
